Common/CExtraction.v
@@ -53,9 +53,6 @@ From Stdlib Require Import ExtrOcamlNativeString.
 From Stdlib Require Import ExtrOcamlZBigInt.
 From Stdlib Require Import ExtrOcamlNatBigInt.
 
-(* Bool.eqb extraction *)
-Extract Inlined Constant Bool.eqb => "(=)".
-
 (* Extract Constant BinNums.PosDef.Pos.add => "Big_int_Z.add_big_int". *)
 
 Extract Inlined Constant map => "Stdlib.List.map".
@@ -64,6 +61,7 @@ Extraction Blacklist String.
 Extraction Blacklist List.
 
 Extract Inlined Constant Decision => "bool".
+
 Extract Inlined Constant Bool.eqb => "(=)".
 
 Extract Inductive fin => "ZO.t"
